high2/Zeta.SeqConsistent.fst
@@ -1,0 +1,106 @@
+module Zeta.SeqConsistent
+
+open FStar.Seq
+open Zeta.Interleave
+open Zeta.App
+open Zeta.Key
+open Zeta.GenKey
+open Zeta.Record
+open Zeta.GenericVerifier
+open Zeta.High.Verifier
+open Zeta.EAC
+open Zeta.Generic.Interleave
+open Zeta.High.Interleave
+
+module V = Zeta.GenericVerifier
+module T = Zeta.Generic.Thread
+module G = Zeta.Generic.Global
+module GI = Zeta.Generic.Interleave
+module HV = Zeta.High.Verifier
+module I = Zeta.Interleave
+module S = FStar.Seq
+module SA = Zeta.SeqAux
+module EAC=Zeta.EAC
+module MSD = Zeta.MultiSetHashDomain
+
+open Zeta.AppSimulate
+open Zeta.AppSimulate.Helper
+
+let lemma_appfn_calls_interleave (#app #n:_) (il: verifiable_log app n)
+  : Lemma (ensures (let cril = appfn_calls_il il in
+                    let gl = to_glog il in
+                    s_seq cril = G.appfn_calls gl))
+          [SMTPat (appfn_calls_il il)]
+  = admit()
+
+let appfn_calls_empty (#app #n:_) (il: verifiable_log app n)
+  : Lemma (ensures (length il = 0 ==> S.length (appfn_calls il) = 0))
+  = admit()
+
+let appfn_calls_snoc (#app #n:_) (il: verifiable_log app n {length il > 0})
+  : Lemma (ensures (let i = length il - 1 in
+                    let e = index il i in
+                    let il' = prefix il i in
+                    let cr = appfn_calls il in
+                    let cr' = appfn_calls il' in
+                    match e with
+                    | RunApp _ _ _ -> cr == SA.append1 cr' (to_appfn_call_res il i)
+                    | _ -> cr == cr'))
+  = admit()
+
+let empty_call_result_valid (#app) (rs: seq (appfn_call_res app))
+  : Lemma (ensures (S.length rs = 0 ==> valid_call_result rs))
+  = admit()
+
+let eac_implies_appfn_valid_empty (#app #n:_) (il: eac_log app n)
+  : Lemma (ensures (length il = 0 ==> valid_call_result (appfn_calls il)))
+  = if length il = 0 then (
+      appfn_calls_empty il;
+      empty_call_result_valid (appfn_calls il)
+    )
+
+let eac_implies_appfn_valid_snoc (#app #n:_) (il: eac_log app n {length il > 0})
+  : Lemma (requires (let i = length il - 1 in
+                     let il' = prefix il i in
+                     valid_call_result (appfn_calls il')))
+          (ensures (valid_call_result (appfn_calls il)))
+  = let i = length il - 1 in
+    let il' = prefix il i in
+    let cr = appfn_calls il in
+    let cr' = appfn_calls il' in
+    let e = index il i in
+    appfn_calls_snoc il;
+
+    match e with
+    | RunApp f p ss -> admit()
+    | _ -> ()
+
+let rec eac_implies_appfn_valid (#app #n:_) (il: eac_log app n)
+  : Lemma (ensures (let cr = appfn_calls il in
+                    valid_call_result cr))
+          (decreases (length il))
+  = eac_implies_appfn_valid_empty il;
+    if length il > 0 then (
+      let i = length il - 1 in
+      let il' = prefix il i in
+      eac_implies_appfn_valid il';
+      eac_implies_appfn_valid_snoc il
+    )
+
+let interleaving_implies_interleave (#a #n:_) (il: interleaving a n)
+  : Lemma (ensures (interleave (i_seq il) (s_seq il)))
+  = let is = i_seq il in
+    let ss = s_seq il in
+    FStar.Classical.exists_intro (fun il -> i_seq il = is /\ s_seq il = ss) il
+
+let lemma_eac_implies_appfn_calls_seq_consistent (#app #n:_) (il: eac_log app n)
+  : Lemma (ensures (let gl = to_glog il in
+                    Zeta.AppSimulate.seq_consistent (G.appfn_calls gl)))
+  = let cr_il = appfn_calls_il il in
+    let crs = i_seq cr_il in
+    let crss = s_seq cr_il in
+    interleaving_implies_interleave cr_il;
+    assert(interleave crs crss);
+    eac_implies_appfn_valid il;
+    assert(valid_call_result crs);
+    FStar.Classical.exists_intro (fun is -> interleave #(appfn_call_res app) is crss) crs
